Cslib/Computability/Distributed/FLP/README.md
@@ -9,6 +9,8 @@ consensus is impossible in the presence of even a single crash fault.
 1. `Algorithm.lean` defines the "syntax" of a distributed algorithm for solving the consensus problem
    and proves some basic properties.
 
+*The following files will appear in future PRs:*
+
 2. `Consensus.lean` defines what it means for a distributed algorithm to solve the consensus problem
    in a fault-tolerant way and proves some basic properties.
 
